Port to new coq-sail register state with stdpp
* The Sail model now uses stdpp bitvectors, although some glue is still
  needed because they're Z-indexed in Sail rather than N-indexed.
* Most of the register handling is now simpler and more uniform
  (e.g., see `sim_simpl_regs`)
* Sail exception handling is slightly different; when we encounter a
  throw we can't just throw away the evaluation context up to the
  handler, but need to accumulate it under a bind first.

sail-riscv/sail_opsem.v
@@ -90,133 +90,56 @@ Lemma byte_to_memory_byte_lookup_Some b i x:
 Proof. do 8 try destruct i => //=; naive_solver lia. Qed.
 
 Definition bv_to_mword {n1 n2} (b : bv n1) : mword n2 :=
-  word_to_mword (Word.NToWord _ (Z.to_N $ bv_unsigned b)).
+  match N.eq_dec n1 (Z.to_N n2) with
+  | left eq => cast_N b eq
+  | right _ => bv_0 _
+  end.
 Arguments bv_to_mword : simpl never.
 Definition mword_to_bv {n1 n2} (b : mword n1) : bv n2 :=
-  default (bv_0 _) (Z_to_bv_checked _ (Z.of_N $ Word.wordToN (get_word b))).
+  match N.eq_dec (Z.to_N n1) n2 with
+  | left eq => cast_N b eq
+  | right _ => bv_0 _
+  end.
 Arguments mword_to_bv : simpl never.
 
 Lemma mword_to_bv_unsigned {n1 n2} (b : mword n1):
   n1 = Z.of_N n2 →
-  bv_unsigned (mword_to_bv (n2:=n2) b) = Z.of_N (Word.wordToN (get_word b)).
+  bv_unsigned (mword_to_bv (n2:=n2) b) = Z.of_N (MachineWord.word_to_N (get_word b)).
 Proof.
-  move => Heq. rewrite /mword_to_bv/Z_to_bv_checked. case_guard as Hn => //=.
-  contradict Hn. apply/bv_wf_in_range. unfold bv_modulus.
-  have /lt_Npow2:= Word.wordToN_bound (get_word b). subst. lia.
-Qed.
-
-Lemma mword_to_bv_signed {n1 n2} (b : mword n1):
-  n1 = Z.of_N n2 →
-  bv_signed (mword_to_bv (n2:=n2) b) = Word.wordToZ (get_word b).
-Proof.
-  move => Heq.
-  rewrite /bv_signed mword_to_bv_unsigned // Word.wordToZ_wordToN /bv_swrap.
-  move: (get_word b) => {}b.
-  destruct (Z.to_nat n1) eqn:?.
-  { rewrite (Word.shatter_word_0 b) /=. have -> : n2 = 0%N by lia. done. }
-  case_match as Hwmsb.
-  - move: Hwmsb => /Word.wmsb_true_bound.
-    rewrite -Npow2_pow. have {1}-> : N.of_nat n = Z.to_N (n1 - 1) by lia.
-    move => /N2Z.inj_le. rewrite N2Z.inj_pow Z2N.id ?ZLib.pow2_div2; [|lia..] => ?.
-    rewrite /bv_wrap (Z.mod_in_range 1).
-    + rewrite /bv_modulus -Npow2_pow N2Z.inj_pow.
-      have -> : N.of_nat (S n) = n2 by lia.
-      lia.
-    + rewrite -bv_half_modulus_twice; [|lia].
-      rewrite /bv_half_modulus /bv_modulus.
-      have -> : Z.of_N n2 = n1 by lia.
-      have := Word.wordToN_bound b.
-      have {2}->: (S n) = Z.to_nat n1 by lia.
-      move => /lt_Npow2 ?.
-      split; try lia.
-      suff : Z.of_N (Word.wordToN b) < (2 ^ n1 `div` 2 + 2 ^ n1 `div` 2) by lia.
-      rewrite Z.add_diag -Z_div_exact_2 //. 1: lia.
-      rewrite Zpow_facts.Zpower_mod // Z.pow_0_l' //. lia.
-  - move: Hwmsb => /Word.wmsb_false_bound.
-    have {2}-> : n = Z.to_nat (n1 - 1) by lia. move => /lt_Npow2.
-    rewrite ZLib.pow2_div2; [|lia] => ?. rewrite bv_wrap_small; [lia|].
-    rewrite -bv_half_modulus_twice; [|lia].
-    rewrite /bv_half_modulus /bv_modulus.
-    have {3}-> : Z.of_N n2 = n1 by lia.
-    lia.
-Qed.
-
-Lemma mword_to_bv_to_mword {n1 n2} (b : bv n1) :
-  n2 = Z.of_N n1 →
-  (@mword_to_bv n2 n1 (bv_to_mword b)) = b.
-Proof.
-  move => Heq. apply bv_eq. rewrite mword_to_bv_unsigned //.
-  rewrite /bv_to_mword/word_to_mword get_word_to_word Word.wordToN_NToWord_2.
-  - bv_saturate. lia.
-  - apply/lt_Npow2; [lia|]. bv_saturate. unfold bv_modulus in *. rewrite Heq. lia.
+  move => Heq. rewrite /mword_to_bv. destruct (N.eq_dec (Z.to_N n1) n2) as [E | NE].
+  - destruct E. rewrite /MachineWord.word_to_N Z2N.id; last apply bv_unsigned_in_range.
+    by rewrite cast_N_refl.
+  - contradict NE. subst; by rewrite N2Z.id.
 Qed.
 
 Lemma uint_plain_to_bv_unsigned n (b : mword n) :
   0 ≤ n →
-  uint b = bv_unsigned (mword_to_bv (n2:=Z.to_N n) b).
-Proof. move => ?. rewrite mword_to_bv_unsigned //. lia. Qed.
+  uint b = bv_unsigned b.
+Proof. move => ?. rewrite /uint/MachineWord.word_to_N Z2N.id //. by apply bv_unsigned_in_range. Qed.
 
-Lemma eq_vec_to_bv n1 {n2} (b1 b2 : mword n2) :
-  n2 = Z.of_N n1 →
-  eq_vec b1 b2 = (bool_decide (mword_to_bv b1 =@{bv n1} mword_to_bv b2)).
+Lemma eq_vec_to_bv n (b1 b2 : mword n) :
+  eq_vec b1 b2 = (bool_decide (b1 = b2)).
 Proof.
-  move => Heq.
   case_bool_decide as Hb.
-  - apply Word.weqb_eq. move: Hb => /bv_eq.
-    by rewrite !mword_to_bv_unsigned // => /N2Z.inj/Word.wordToN_inj.
-  - apply Word.weqb_ne. contradict Hb. apply bv_eq.
-    by rewrite !mword_to_bv_unsigned // Hb.
+  - rewrite eq_vec_true_iff //.
+  - rewrite eq_vec_false_iff //.
 Qed.
 
-Lemma unfold_machineword_slice m n (w : Word.word m) i :
-  forall H : (i + n <= m)%nat,
-  MachineWord.slice n w i = let w0 := TypeCasts.cast_nat w (MachineWord.MachineWord.slice_equality H) in Word.split1 n (m - n - i) (Word.split2 i (n + (m - n - i)) w0).
-intros.
-unfold MachineWord.slice.
-destruct (le_lt_dec (i + n) m).
-* rewrite (le_unique _ _ H l).
-  reflexivity.
-* lia.
-Qed.
-
-Lemma mword_to_bv_subrange_vec_dec z1 z2 n2 n1 (b : mword n1):
-  0 <= z2 ->
-  z2 <= z1 < n1 ->
-  n1 = Z.of_N n2 →
-  mword_to_bv (subrange_vec_dec b z1 z2) =
-    bv_extract (Z.to_N z2) (Z.to_N (z1 + 1 - z2)) (mword_to_bv (n2:=n2) b).
+Lemma N_eq_dec_eq m n (E : m = n) :
+  N.eq_dec m n = left E.
 Proof.
-  move => Hz2 Hz1 ?.
-  unfold subrange_vec_dec.
-  apply bv_eq.
-  rewrite bv_extract_unsigned !mword_to_bv_unsigned; [|lia..].
-
-  have ZNAT : (Z.to_nat z1 - Z.to_nat z2 + 1 = Z.to_nat (z1 - z2 + 1))%nat by lia.
-  rewrite ZNAT.
-
-  rewrite -to_word_to_word_nat; [|lia].
-  rewrite get_word_to_word.
-
-  rewrite unfold_machineword_slice; [lia|]. move => ?.
-  rewrite wordToN_split1 wordToN_split2 wordToN_cast_word.
-
-  rewrite !Z_nat_N !Z2N.id ?N2Z.inj_div ?N2Z.inj_mod ?N2Z.inj_pow ?Z2N.id; [|lia..].
-  rewrite N2Z.inj_div N2Z.inj_pow Z2N.id // -Z.shiftr_div_pow2 -?Z.land_ones; [|lia..].
-  bitblast.
+  destruct (N.eq_dec m n).
+  - f_equal. apply Eqdep_dec.UIP_dec. apply N.eq_dec.
+  - exfalso. congruence.
 Qed.
-
-Lemma get_bit_get_word_testbit n z (w : mword n):
-  (z < Z.to_nat n)%nat →
-  MachineWord.get_bit (get_word w) z = Z.testbit (bv_unsigned (mword_to_bv (n2:=Z.to_N n) w)) (Z.of_nat z).
-Proof. etrans; [apply getBit_testbit|]; [lia|]. rewrite mword_to_bv_unsigned //. lia. Qed.
 
 Lemma access_vec_dec_to_bv  n1 (b : mword n1) z :
   0 ≤ z →
   z < n1 →
   access_vec_dec b z = bitU_of_bool (Z.testbit (bv_unsigned (mword_to_bv (n2:=Z.to_N n1) b)) z).
 Proof.
-  move => ??. rewrite /access_vec_dec/access_mword_dec. f_equal. rewrite get_bit_get_word_testbit => //.
-  1:f_equal. all: lia.
+  move => ??. rewrite /access_vec_dec/access_mword_dec/MachineWord.get_bit/MachineWord.Z_idx Z2N.id /mword_to_bv; last lia.
+  rewrite N_eq_dec_eq cast_N_refl /get_word //.
 Qed.
 
 Lemma mword_to_bv_add_vec {n1 : Z} {n2 : N} (b1 b2 : mword n1) :
@@ -225,64 +148,15 @@ Lemma mword_to_bv_add_vec {n1 : Z} {n2 : N} (b1 b2 : mword n1) :
 Proof.
   move => Hn. apply bv_eq.
   rewrite bv_add_unsigned !mword_to_bv_unsigned // get_word_word_binop.
-  rewrite /Word.wplus /Word.wordBin Word.wordToN_NToWord_eqn.
-  rewrite /bv_wrap/bv_modulus -(N2Z.inj_pow 2) -Npow2_pow Z_nat_N.
-  rewrite N2Z.inj_mod N2Z.inj_add. f_equal. by rewrite Hn N2Z.id.
+  rewrite /MachineWord.word_to_N/MachineWord.add/get_word.
+  rewrite !Z2N.id; [ | apply bv_unsigned_in_range..].
+  unfold mword, MachineWord.word, MachineWord.Z_idx in *.
+  subst.
+  rewrite N2Z.id in b2, b1 |- *.
+  bv_solve.
 Qed.
 Arguments add_vec : simpl never.
 
-Lemma mword_to_bv_add_vec_int n1 n2 (b : mword n1) z:
-  0 ≤ z → (* not strictly necessary but makes the proof easier *)
-  n1 = Z.of_N n2 →
-  mword_to_bv (n2:=n2) (add_vec_int b z) = bv_add_Z (mword_to_bv b) z.
-Proof.
-  move => ??.
-  rewrite /add_vec_int mword_to_bv_add_vec //.
-  apply bv_eq.
-  rewrite bv_add_unsigned bv_add_Z_unsigned.
-  rewrite -(bv_wrap_add_idemp_r _ _ z).
-  f_equal. f_equal.
-  rewrite mword_to_bv_unsigned // get_word_mword_of_int.
-  rewrite -Word.NToWord_Z_to_N // Word.wordToN_NToWord_eqn -Npow2_pow Z_nat_N.
-  rewrite N2Z.inj_mod N2Z.inj_pow !Z2N.id; [|lia..].
-  unfold bv_wrap, bv_modulus in *.
-  do 2 f_equal. done.
-Qed.
-
-Lemma unfold_sign_extend m n (w: Word.word m) :
-  forall H : (m <= n)%nat,
-  MachineWord.sign_extend n w = cast_nat (Word.sext w (n - m)) (MachineWord.MachineWord.extend_ok H).
-Proof.
-  intro.
-  rewrite /MachineWord.sign_extend.
-  destruct (le_lt_dec m n).
-  * rewrite (le_unique m n H) //.
-  * lia.
-Qed.
-
-Lemma wordToZ_cast_nat m n (E : m = n) w :
-  Word.wordToZ (cast_nat w E) = Word.wordToZ w.
-Proof.
-  subst.
-  rewrite cast_nat_refl.
-  reflexivity.
-Qed.
-
-Lemma mword_to_bv_sign_extend' n1 n2' n2 (b : mword n1):
-  0 ≤ n1 →
-  n2' = Z.of_N n2 →
-  n1 ≤ n2' →
-  mword_to_bv (n2:=n2) (sign_extend' n2' b) = bv_sign_extend _ (mword_to_bv (n2:=(Z.to_N n1)) b).
-Proof.
-  move => ???.
-  apply bv_eq_signed. rewrite mword_to_bv_signed //. rewrite /sign_extend'/sign_extend/exts_vec/= get_word_to_word.
-  rewrite unfold_sign_extend. 1: lia. move => ?. rewrite wordToZ_cast_nat.
-  rewrite Word.sext_wordToZ bv_sign_extend_signed ?mword_to_bv_signed //.
-  all: lia.
-Qed.
-Global Arguments sign_extend' : simpl never.
-
-(* #[local] Hint Rewrite wordToN_spec_high Z_of_bool_spec_high using lia : rewrite_bits_db. *)
 Lemma mword_to_bv_update_vec_dec n1 n2 (b : mword n1) b1 z b2:
   bool_of_bitU b1 = Some b2 →
   n1 = Z.of_N n2 →
@@ -295,144 +169,32 @@ Proof.
   move => Hb ???.
   apply bv_eq. rewrite mword_to_bv_unsigned //.
   rewrite /update_vec_dec/opt_def /update_mword_dec Hb.
-  rewrite /update_mword_bool_dec get_word_with_word wordToN_setBit;[|lia..].
+  rewrite /update_mword_bool_dec get_word_with_word wordToN_setBit/MachineWord.Z_idx;[|lia].
   rewrite bv_or_unsigned bv_and_unsigned bv_not_unsigned !Z_to_bv_unsigned mword_to_bv_unsigned//.
-  rewrite Z2Nat.id; [|lia]. rewrite !bv_wrap_land.
+  rewrite /MachineWord.word_to_N/get_word.
+  unfold mword, MachineWord.word, MachineWord.Z_idx in b.
+  rewrite !Z2N.id; [|by apply bv_unsigned_in_range|lia].
+ rewrite !bv_wrap_land.
   bitblast.
 Qed.
 
-Lemma mem_bytes_of_bits_to_bv n (v : mword n) len:
-  n = 8 * len →
-  0 <= n →
-  mem_bytes_of_bits v = Some (byte_to_memory_byte <$>
-       (bv_to_little_endian len 8 (@bv_unsigned (Z.to_N n) (mword_to_bv v)))).
-Proof.
-  move => Hn ?.
-  rewrite /mem_bytes_of_bits/bytes_of_bits/bits_of/= option_map_fmap map_fmap.
-  apply fmap_Some. eexists (rev _). rewrite rev_involutive. split; [|done].
-  rewrite (byte_chunks_reshape (Z.to_nat len)).
-  2: { rewrite fmap_length MachineWord.word_to_bools_length. lia. }
-  f_equal. eapply list_eq_same_length; [done | |].
-  { rewrite reshape_length rev_length replicate_length fmap_length bv_to_little_endian_length; lia. }
-  move => i x y ?. rewrite rev_reverse sublist_lookup_reshape; [|lia|].
-  2: { rewrite fmap_length MachineWord.word_to_bools_length. lia. }
-  move => /sublist_lookup_Some'[??] /reverse_lookup_Some.
-  rewrite list_lookup_fmap fmap_length bv_to_little_endian_length; [|lia] => -[Hl ?].
-  move: Hl => /fmap_Some[?[/bv_to_little_endian_lookup_Some[|???]]]; [lia|]. simplify_eq.
-  apply: list_eq_same_length; [done|..].
-  { rewrite byte_to_memory_byte_length take_length_le ?drop_length; lia. }
-  move => i' x y ? /lookup_take_Some. rewrite lookup_drop list_lookup_fmap.
-  have H : (Z.to_nat (8 * len) > 0)%nat by lia.
-  move => [/fmap_Some[?[/(word_to_bools_lookup_Some _ _ _ _ H)[??]?]]?] /byte_to_memory_byte_lookup_Some[??].
-  simplify_eq. f_equal.
-  rewrite -(mword_to_bv_unsigned (n2:=(Z.to_N (8 * len)))); [|lia].
-  rewrite Z_to_bv_unsigned bv_wrap_spec_low ?Z.shiftr_spec; [|lia..].
-  f_equal. lia.
-Qed.
-
-Lemma just_list_bits_of_mem_bytes bs:
-  just_list (bool_of_bitU <$> bits_of_mem_bytes (byte_to_memory_byte <$> bs)) =
-    Some (mjoin (((λ x, reverse (bv_to_bits x)) <$> reverse bs))).
-Proof.
-  rewrite just_list_mapM. apply mapM_Some_2. apply Forall2_same_length_lookup_2. {
-    rewrite fmap_length join_length -list_fmap_compose /compose /= sum_list_fmap_const.
-    rewrite length_bits_of_mem_bytes ?fmap_length ?reverse_length //.
-    move => ? /elem_of_list_fmap[?[??]]. subst. by rewrite byte_to_memory_byte_length.
-  }
-  move => i x y. rewrite list_lookup_fmap /bits_of_mem_bytes/bits_of_bytes concat_join map_fmap.
-  move => /fmap_Some[?[/(join_lookup_Some_same_length 8)[|?[?[?[Hm [Hl ?]]]]]]].
-  { apply list.Forall_forall => ?. rewrite rev_reverse. move => /elem_of_list_fmap[?[? /elem_of_reverse /elem_of_list_fmap[?[??]]]]; subst. done. }
-  move => ?. subst. move: Hm. rewrite list_lookup_fmap rev_reverse. move => /fmap_Some [?[Hrev ?]]. subst.
-  move: Hl. rewrite /bits_of /= map_fmap list_lookup_fmap => /fmap_Some [?[Hl ?]]. subst.
-  move: Hrev => /reverse_lookup_Some. rewrite list_lookup_fmap => -[/fmap_Some[?[Hbs ?]] ?]. subst.
-  move: Hl => /byte_to_memory_byte_lookup_Some[??].
-  move => /join_lookup_Some_same_length'[| |].
-  { apply list.Forall_forall => ? /elem_of_list_fmap[?[??]]. subst. by rewrite reverse_length bv_to_bits_length. }
-  { done. }
-  move => ?. rewrite list_lookup_fmap => -[/fmap_Some[?[/reverse_lookup_Some[??] ?]] Hl].
-  rewrite fmap_length in Hbs; simplify_eq.
-  move: Hl => /reverse_lookup_Some [/bv_to_bits_lookup_Some[??] ?]; simplify_eq.
-  by rewrite bool_of_bitU_of_bool bv_to_bits_length.
-Qed.
-
-Lemma wordToN_cast_nat m n w (E: m = n) :
-  Word.wordToN (cast_nat w E) = Word.wordToN w.
-subst.
-rewrite cast_nat_refl.
-reflexivity.
-Qed.
-
-Lemma read_mem_bytes_eq (len' : N) n bs:
-  n = (length bs * 8) →
-  len' = N.of_nat (length bs) →
-     of_bits (n:=n) (bits_of_mem_bytes (byte_to_memory_byte <$> bs)) = Some
-     (bv_to_mword (Z_to_bv (8 * len') (little_endian_to_bv 8 bs))).
-Proof.
-  move => ??.
-  have n_pos : n >=? 0 = true by lia.
-  rewrite /of_bits just_list_bits_of_mem_bytes.
-  match goal with |- match ?e with | _ => _ end = _ => destruct e as [Hhyp|Hhyp] end. 2: {
-    rewrite /length_list join_length -list_fmap_compose /compose /= (sum_list_fmap_same 8) ?reverse_length in Hhyp; [lia|].
-    by apply Forall_true.
-  }
-  f_equal.
-  apply get_word_inj. rewrite !get_word_to_word cast_Z_id.
-  destruct Hhyp => /=. apply Word.wordToN_inj.
-  rewrite Word.wordToN_NToWord_2. 2: {
-    rewrite -Npow2_pow Z_to_bv_unsigned /length_list join_length Nat2Z.id -list_fmap_compose /compose /= (sum_list_fmap_same 8) ?reverse_length; [|by apply Forall_true].
-    have ? := bv_wrap_in_range (8 * len') (little_endian_to_bv 8 bs).
-    unfold bv_modulus in *.
-    apply N2Z.inj_lt.
-    have ->: N.of_nat (length bs * 8) = (8 * len')%N by lia.
-    rewrite N2Z.inj_pow. lia.
-  }
-  apply N2Z.inj. rewrite Z2N.id. 2: {
-    have ? := bv_unsigned_in_range _ (Z_to_bv (8 * len') (little_endian_to_bv 8 bs)). lia.
-  }
-  rewrite Z_to_bv_unsigned. apply Z.bits_inj_iff' => i ?.
-  have {1}->: i = Z.of_nat (Z.to_nat i) by lia.
-  rewrite get_word_to_word wordToN_cast_nat.
-  rewrite bools_to_word_spec rev_reverse.
-  rewrite bv_wrap_spec //. case_bool_decide => /=.
-  2: { rewrite lookup_ge_None_2 // reverse_length join_length -list_fmap_compose /compose /= (sum_list_fmap_same 8) ?reverse_length; [lia|]. by apply Forall_true. }
-  rewrite /default. case_match as Hc.
-  2: { rewrite lookup_ge_None reverse_length join_length -list_fmap_compose /compose /= (sum_list_fmap_same 8) ?reverse_length in Hc; [lia|]. by apply Forall_true. }
-  move: Hc => /reverse_lookup_Some [/(join_lookup_Some_same_length 8)[|j1 [?[j2[Hl[Hl2 Hi]]]] ?]]. {
-    apply Forall_forall => ? /elem_of_list_fmap[?[??]]. subst.
-    by rewrite reverse_length bv_to_bits_length.
-  }
-  move: Hi => /Nat2Z.inj_iff. rewrite join_length -list_fmap_compose /compose /= (sum_list_fmap_same 8) ?reverse_length.
-  2: { by apply Forall_forall. }
-  move => Hi.
-  have {Hi} ?: i = (length bs * 8 - 1 - (j1 * 8 + j2))%nat by lia. simplify_eq.
-  move: Hl. rewrite list_lookup_fmap => /fmap_Some[?[/reverse_lookup_Some[Hbs ?] ?]]. simplify_eq.
-  move: Hl2  => /reverse_lookup_Some[/bv_to_bits_lookup_Some[??]?]. simplify_eq/=.
-  erewrite little_endian_to_bv_spec; [|lia|done|]. 2: { erewrite <-Hbs. f_equal. lia. }
-  f_equal. lia.
-Qed.
-
-Definition register_value_to_valu (r : register_name) (v : register_value) : valu :=
-  if bool_decide (r = "misa" ∨ r = "mstatus") then
-    if v is Regval_bitvector_64 m then
-      RegVal_Struct [("bits", RVal_Bits (mword_to_bv (n2:=64) m))]
-    else
-      RegVal_Poison
-  else
-  match v with
-  | Regval_bitvector_1 m => RVal_Bits (mword_to_bv (n2:=1) m)
-  | Regval_bitvector_2 m => RVal_Bits (mword_to_bv (n2:=2) m)
-  | Regval_bitvector_3 m => RVal_Bits (mword_to_bv (n2:=3) m)
-  | Regval_bitvector_4 m => RVal_Bits (mword_to_bv (n2:=4) m)
-  | Regval_bitvector_8 m => RVal_Bits (mword_to_bv (n2:=8) m)
-  | Regval_bitvector_16 m => RVal_Bits (mword_to_bv (n2:=16) m)
-  | Regval_bitvector_32 m => RVal_Bits (mword_to_bv (n2:=32) m)
-  | Regval_bitvector_64 m => RVal_Bits (mword_to_bv (n2:=64) m)
-  | Regval_bitvector_65536 m => RVal_Bits (mword_to_bv (n2:=65536) m)
-  | Regval_bool b => RVal_Bool b
-  | Regval_Privilege p => RVal_Enum (match p with | User => "User" | Supervisor => "Supervisor" | Machine => "Machine" end)
-  | _ => RegVal_Poison
+Definition register_value_to_valu {T} (r : register T) :  T -> valu :=
+  match r with
+  | R_bitvector_64 misa => fun m => RegVal_Struct [("bits", RVal_Bits (mword_to_bv (n2:=64) m))]
+  | R_bitvector_64 mstatus => fun m => RegVal_Struct [("bits", RVal_Bits (mword_to_bv (n2:=64) m))]
+  | R_bitvector_1 _ => fun m => RVal_Bits (mword_to_bv (n2:=1) m)
+  | R_bitvector_2 _ => fun m => RVal_Bits (mword_to_bv (n2:=2) m)
+  | R_bitvector_3 _ => fun m => RVal_Bits (mword_to_bv (n2:=3) m)
+  | R_bitvector_4 _ => fun m => RVal_Bits (mword_to_bv (n2:=4) m)
+  | R_bitvector_16 _ => fun m => RVal_Bits (mword_to_bv (n2:=16) m)
+  | R_bitvector_32 _ => fun m => RVal_Bits (mword_to_bv (n2:=32) m)
+  | R_bitvector_64 _ => fun m => RVal_Bits (mword_to_bv (n2:=64) m)
+  | R_bitvector_65536 _ => fun m =>  RVal_Bits (mword_to_bv (n2:=65536) m)
+  | R_bool _ => fun b => RVal_Bool b
+  | R_Privilege _ => fun p => RVal_Enum (match p with | User => "User" | Supervisor => "Supervisor" | Machine => "Machine" end)
+  | _ => fun _ => RegVal_Poison
   end.
-Global Arguments register_value_to_valu !_ !_ /.
+Global Arguments register_value_to_valu {_} !_ !_ /.
 
 Lemma iris_module_wf_isla_lang :
   iris_module_wf isla_lang.
@@ -457,62 +219,56 @@ Definition instruction_length (i : encoded_instruction) : mword 64 :=
    end.
 
 Definition step_cpu (i : encoded_instruction) : M () :=
-  (match i with
+  dec ← (match i with
    | Uncompressed ie => riscv.encdec_backwards (bv_to_mword ie)
    | Compressed ie => riscv.encdec_compressed_backwards (bv_to_mword ie)
-   end) >>= λ dec,
-   read_reg PC_ref >>= λ PC,
-   write_reg nextPC_ref (add_vec PC (instruction_length i)) >>
-   execute dec >>= λ R, if R is RETIRE_SUCCESS then
-                          read_reg nextPC_ref >>= λ nextPC,
-                          write_reg PC_ref nextPC >>
-                          Done tt
+   end);
+   PC_val ← Defs.read_reg PC;
+   Defs.write_reg nextPC (add_vec PC_val (instruction_length i));;
+   R ← execute dec;  if R is RETIRE_SUCCESS then
+                          nextPC ← Defs.read_reg nextPC;
+                          Defs.write_reg PC nextPC
                         else
-                          Fail "execution failed!".
+                          fail "execution failed!".
 
+Import Interface.
 
 Inductive sail_step : sail_state → option seq_label → sail_state → Prop :=
 | SailDone rs h i ins :
-  ins !! mword_to_bv (PC rs) = Some i →
-  sail_step (SAIL (Done tt) rs h ins false) None (SAIL (step_cpu i) rs h ins false)
+  ins !! mword_to_bv (register_lookup PC rs) = Some i →
+  sail_step (SAIL (Ret tt) rs h ins false) None (SAIL (step_cpu i) rs h ins false)
 | SailStop rs h ins :
-  ins !! mword_to_bv (PC rs) = None →
-  sail_step (SAIL (Done tt) rs h ins false) (Some (SInstrTrap (mword_to_bv (PC rs)))) (SAIL (Done tt) rs h ins true)
-| SailChoose rs h ins ty e s v:
-  sail_step (SAIL (Choose s ty e) rs h ins false) None (SAIL (e v) rs h ins false)
-| SailReadReg rs h ins e r v:
-  get_regval r rs = Some v →
-  sail_step (SAIL (Read_reg r e) rs h ins false) None (SAIL (e v) rs h ins false)
-| SailWriteReg rs rs' h ins e r v:
-  set_regval r v rs = Some rs' →
-  sail_step (SAIL (Write_reg r v e) rs h ins false) None (SAIL e rs' h ins false)
-| SailReadMem rs h ins e a bs' sz κ adr len:
-  adr = (Z_to_bv 64 (Z.of_N a)) →
-  (len = N.of_nat sz)%N →
-  length bs' = sz →
-  (if read_mem_list h (Z.of_N a) len is Some bs then
+  ins !! mword_to_bv (register_lookup PC rs) = None →
+  sail_step (SAIL (Ret tt) rs h ins false) (Some (SInstrTrap (mword_to_bv (register_lookup PC rs)))) (SAIL (Ret tt) rs h ins true)
+| SailChoose rs h ins ty e v:
+  sail_step (SAIL (Next (Choose ty) e) rs h ins false) None (SAIL (e v) rs h ins false)
+| SailReadReg T rs h ins e (r : register T) ak v:
+  register_lookup r rs = v →
+  sail_step (SAIL (Next (RegRead r ak) e) rs h ins false) None (SAIL (e v) rs h ins false)
+| SailWriteReg T rs rs' h ins e (r : register T) ak v:
+  register_set r v rs = rs' →
+  sail_step (SAIL (Next (RegWrite r ak v) e) rs h ins false) None (SAIL (e tt) rs' h ins false)
+| SailReadMem rs h ins κ len bs' req e:
+  (if read_mem_list h (bv_unsigned req.(ReadReq.pa)) len is Some bs then
     κ = None ∧
-    bs = bs'
+    Z_to_bv (8 * len) (little_endian_to_bv 8 bs) = bs'
   else
-    Z.of_N a + Z.of_N len ≤ 2 ^ 64 ∧
-    set_Forall (λ ad, ¬ (Z.of_N a ≤ bv_unsigned ad < Z.of_N a + Z.of_N len)) (dom h) ∧
-    κ = Some (SReadMem adr (Z_to_bv (8 * len) (little_endian_to_bv 8 bs')))) →
-  sail_step (SAIL (Read_mem Read_plain a sz e) rs h ins false) κ (SAIL (e (byte_to_memory_byte <$> bs')) rs h ins false)
-| SailWriteMem rs h h' ins e a bs bs' sz len adr κ:
-  adr = (Z_to_bv 64 (Z.of_N a)) →
-  (len = N.of_nat sz)%N →
-  bs = byte_to_memory_byte <$> bs' →
-  (if read_mem_list h (Z.of_N a) len is Some _ then
-    write_mem_list h (Z_to_bv 64 (Z.of_N a)) bs' = h' ∧
+    bv_unsigned req.(ReadReq.pa) + Z.of_N len ≤ 2 ^ 64 ∧
+    set_Forall (λ ad, ¬ (bv_unsigned req.(ReadReq.pa) ≤ bv_unsigned ad < bv_unsigned req.(ReadReq.pa) + Z.of_N len)) (dom h) ∧
+    κ = Some (SReadMem req.(ReadReq.pa) bs')) →
+  sail_step (SAIL (Next (MemRead len req) e) rs h ins false) κ (SAIL (e (inl (bs', None))) rs h ins false)
+| SailWriteMem rs h h' ins e len req κ:
+  (if read_mem_list h (bv_unsigned req.(WriteReq.pa)) len is Some _ then
+    write_mem len h req.(WriteReq.pa) (bv_unsigned req.(WriteReq.value)) = h' ∧
     κ = None
   else
-    Z.of_N a + Z.of_N len ≤ 2 ^ 64 ∧
-    set_Forall (λ ad, ¬ (Z.of_N a ≤ bv_unsigned ad < Z.of_N a + Z.of_N len)) (dom h) ∧
+    bv_unsigned req.(WriteReq.pa) + Z.of_N len ≤ 2 ^ 64 ∧
+    set_Forall (λ ad, ¬ (bv_unsigned req.(WriteReq.pa) ≤ bv_unsigned ad < bv_unsigned req.(WriteReq.pa) + Z.of_N len)) (dom h) ∧
     h = h' ∧
-    κ = Some (SWriteMem adr (Z_to_bv (8 * len) (little_endian_to_bv 8 bs')))) →
-  sail_step (SAIL (Write_mem Write_plain a sz bs e) rs h ins false) κ (SAIL (e true) rs h' ins false)
-| SailWriteEa rs h ins e wk n1 n2:
-  sail_step (SAIL (Write_ea wk n1 n2 e) rs h ins false) None (SAIL e rs h ins false)
+    κ = Some (SWriteMem req.(WriteReq.pa) req.(WriteReq.value))) →
+  sail_step (SAIL (Next (MemWrite len req) e) rs h ins false) κ (SAIL (e (inl None)) rs h' ins false)
+(*| SailWriteEa rs h ins e wk n1 n2:
+  sail_step (SAIL (Write_ea wk n1 n2 e) rs h ins false) None (SAIL e rs h ins false)*)
 .
 
 Definition sail_module := {|
@@ -523,59 +279,59 @@ Definition sail_module := {|
 (*** [mctx]: Evaluation contexts for [monad] *)
 Inductive mctx : Type → Type → Type :=
 | NilMCtx : mctx () exception
-| BindMCtx {A1 A2 E} (f : A1 → monad register_value A2 E) (K : mctx A2 E) : mctx A1 E
-| TryMCtx {A E1 E2} (f : E1 → monad register_value A E2) (K : mctx A E2) : mctx A E1.
+| BindMCtx {A1 A2 E} (f : A1 → monad E A2) (K : mctx A2 E) : mctx A1 E
+| TryMCtx {A E1 E2} (f : E1 → monad E2 A) (K : mctx A E2) : mctx A E1.
 
-Fixpoint mctx_interp {A E} (K : mctx A E) : monad register_value A E → M () :=
-  match K in (mctx A' E') return (monad register_value A' E' → M _) with
+Fixpoint mctx_interp {A E} (K : mctx A E) : monad E A → M () :=
+  match K in (mctx A' E') return (monad E' A' → M _) with
    | NilMCtx => λ e, e
    | BindMCtx f K => λ e, mctx_interp K (e >>= f)
    | TryMCtx f K => λ e, mctx_interp K (try_catch e f)
    end.
 
-Lemma mctx_interp_Choose A E K s choose_ty e1:
-  @mctx_interp A E K (Choose s choose_ty e1) = Choose s choose_ty (λ v, mctx_interp K (e1 v)).
+Lemma mctx_interp_Choose A E K choose_ty e1:
+  @mctx_interp A E K (Next (Choose choose_ty) e1) = Next (Choose choose_ty) (λ v, mctx_interp K (e1 v)).
 Proof. elim: K e1 => //=. Qed.
-Lemma mctx_interp_Read_reg A E K r e1:
-  @mctx_interp A E K (Read_reg r e1) = Read_reg r (λ v, mctx_interp K (e1 v)).
+Lemma mctx_interp_Read_reg T A E K (r : register T) ak e1:
+  @mctx_interp A E K (Next (RegRead r ak) e1) = Next (RegRead r ak) (λ v, mctx_interp K (e1 v)).
 Proof. elim: K e1 => //=. Qed.
-Lemma mctx_interp_Write_reg A E K r e1 v:
-  @mctx_interp A E K (Write_reg r v e1) = Write_reg r v (mctx_interp K e1).
+Lemma mctx_interp_Write_reg T A E K (r : register T) ak e1 v:
+  @mctx_interp A E K (Next (RegWrite r ak v) e1) = Next (RegWrite r ak v) (λ v, mctx_interp K (e1 v)).
 Proof. elim: K e1 => //=. Qed.
-Lemma mctx_interp_Read_mem A E K e1 a sz rk:
-  @mctx_interp A E K (Read_mem rk a sz e1) = Read_mem rk a sz (λ v, mctx_interp K (e1 v)).
+Lemma mctx_interp_Read_mem A E K sz req e1:
+  @mctx_interp A E K (Next (MemRead sz req) e1) = Next (MemRead sz req) (λ v, mctx_interp K (e1 v)).
 Proof. elim: K e1 => //=. Qed.
-Lemma mctx_interp_Write_mem A E K e1 a sz bs wk:
-  @mctx_interp A E K (Write_mem wk a sz bs e1) = Write_mem wk a sz bs (λ v, mctx_interp K (e1 v)).
+Lemma mctx_interp_Write_mem A E K sz req e1:
+  @mctx_interp A E K (Next (MemWrite sz req) e1) = Next (MemWrite sz req) (λ v, mctx_interp K (e1 v)).
 Proof. elim: K e1 => //=. Qed.
-Lemma mctx_interp_Write_ea A E K n1 n2 wk e1:
+(*Lemma mctx_interp_Write_ea A E K n1 n2 wk e1:
   @mctx_interp A E K (Write_ea wk n1 n2 e1) = Write_ea wk n1 n2 (mctx_interp K e1).
-Proof. elim: K e1 => //=. Qed.
+Proof. elim: K e1 => //=. Qed.*)
 
 (*** [sim]: Simulation relation *)
-Definition get_plat_config (reg_name : string) : option register_value :=
+Definition get_plat_config (reg_name : string) : option valu :=
   match reg_name with
-  | "rv_enable_pmp" => Some (Regval_bool (plat_enable_pmp ()))
-  | "rv_enable_misaligned_access" => Some (Regval_bool (plat_enable_misaligned_access ()))
-  | "rv_ram_base" => Some (Regval_bitvector_64 (plat_ram_base ()))
-  | "rv_ram_size" => Some (Regval_bitvector_64 (plat_ram_size ()))
-  | "rv_rom_base" => Some (Regval_bitvector_64 (plat_rom_base ()))
-  | "rv_rom_size" => Some (Regval_bitvector_64 (plat_rom_size ()))
-  | "rv_clint_base" => Some (Regval_bitvector_64 (plat_clint_base ()))
-  | "rv_clint_size" => Some (Regval_bitvector_64 (plat_clint_size ()))
-  | "rv_htif_tohost" => Some (Regval_bitvector_64 (plat_htif_tohost ()))
-  | "Machine" => Some (Regval_Privilege (Machine))
+  | "rv_pmp_count" => Some (RegVal_I (sys_pmp_count ()) 64)
+  | "rv_enable_misaligned_access" => Some (RVal_Bool (plat_enable_misaligned_access ()))
+  | "rv_ram_base" => Some (RVal_Bits (mword_to_bv (n2:=64) (plat_ram_base ())))
+  | "rv_ram_size" => Some (RVal_Bits (mword_to_bv (n2:=64) (plat_ram_size ())))
+  | "rv_rom_base" => Some (RVal_Bits (mword_to_bv (n2:=64) (plat_rom_base ())))
+  | "rv_rom_size" => Some (RVal_Bits (mword_to_bv (n2:=64) (plat_rom_size ())))
+  | "rv_clint_base" => Some (RVal_Bits (mword_to_bv (n2:=64) (plat_clint_base ())))
+  | "rv_clint_size" => Some (RVal_Bits (mword_to_bv (n2:=64) (plat_clint_size ())))
+  | "rv_htif_tohost" => Some (RVal_Bits (mword_to_bv (n2:=64) (plat_htif_tohost ())))
+  | "Machine" => Some (RVal_Enum "Machine")
   | _ => None
   end.
 
-Definition get_regval_or_config (reg_name : string) (s : regstate) : option register_value :=
-  match get_regval reg_name s with
-  | Some v => Some v
+Definition get_regval_or_config (reg_name : string) (s : regstate) : option valu :=
+  match register_of_string reg_name with
+  | Some (GRegister.GReg r) => Some (register_value_to_valu r (register_lookup r s))
   | None => get_plat_config reg_name
   end.
 
 Definition isla_regs_wf (regs : regstate) (isla_regs : reg_map) : Prop :=
-  ∀ r vi, isla_regs !! r = Some vi → ∃ vs, get_regval_or_config r regs = Some vs ∧ vi = (register_value_to_valu r vs).
+  ∀ r vi, isla_regs !! r = Some vi → get_regval_or_config r regs = Some vi. 
 
 Definition private_regs_wf (isla_regs : reg_map) : Prop :=
   isla_regs !! "nextPC" = None.
@@ -586,7 +342,7 @@ Record sim_state := SIM {
 Add Printing Constructor sim_state.
 Global Instance eta_sim_state : Settable _ := settable! SIM <sim_regs>.
 
-Definition sim {A E} (Σ : sim_state) (e1 : monad register_value A E) (K : mctx A E) (e2 : isla_trace) : Prop :=
+Definition sim {A E} (Σ : sim_state) (e1 : monad E A) (K : mctx A E) (e2 : isla_trace) : Prop :=
   ∀ n isla_regs mem sail_instrs isla_instrs,
   isla_regs_wf Σ.(sim_regs) isla_regs →
   private_regs_wf isla_regs →
@@ -595,7 +351,7 @@ Definition sim {A E} (Σ : sim_state) (e1 : monad register_value A E) (K : mctx 
       private_regs_wf isla_regs' →
       dom isla_regs' = dom isla_regs →
       raw_sim sail_module (iris_module isla_lang) n
-          (SAIL (Done tt) sail_regs' mem' sail_instrs false)
+          (SAIL (Ret tt) sail_regs' mem' sail_instrs false)
           ({| seq_trace := tnil; seq_regs := isla_regs'; seq_nb_state := false; seq_pc_reg := arch_pc_reg|},
            {| seq_instrs := isla_instrs; seq_mem := mem' |})) →
   raw_sim sail_module (iris_module isla_lang) n
@@ -611,20 +367,20 @@ Lemma sim_implies_refines sail_instrs isla_instrs sail_regs isla_regs mem :
   isla_regs_wf sail_regs isla_regs →
   private_regs_wf isla_regs →
   (∀ a si ii, sail_instrs !! a = Some si → isla_instrs !! a = Some ii → sim_instr si ii) →
-  refines sail_module (SAIL (Done tt) sail_regs mem sail_instrs false)
+  refines sail_module (SAIL (Ret tt) sail_regs mem sail_instrs false)
           (iris_module isla_lang) (initial_local_state isla_regs, {| seq_instrs := isla_instrs; seq_mem := mem |}).
 Proof.
   move => Hdom Hregs Hpriv Hsim. apply: raw_sim_implies_refines => n.
   elim/lt_wf_ind: n sail_regs isla_regs mem Hregs Hpriv.
   move => n IH sail_regs isla_regs mem Hregs Hpriv.
   apply: raw_sim_safe_here => /= Hsafe.
-  have {Hsafe} ? : isla_regs !! "PC" = Some (RVal_Bits (mword_to_bv (n2:=64) (PC sail_regs))). {
+  have {Hsafe} ? : isla_regs !! "PC" = Some (RVal_Bits (mword_to_bv (n2:=64) (register_lookup PC sail_regs))). {
     destruct (isla_regs !! "PC") eqn: HPC.
-    - have [? [[<-] ->]]:= Hregs "PC" _ ltac:(done). done.
+    - have [<-]:= Hregs "PC" _ ltac:(done). done.
     - move: Hsafe => [[]|]// [?[?[?[? Hsafe]]]]. inv_seq_step.
       revert select (∃ x, _) => -[?[??]]; unfold sail_name in *; simplify_eq.
   }
-  destruct (sail_instrs !! mword_to_bv (PC sail_regs)) as [si|] eqn: Hsi.
+  destruct (sail_instrs !! mword_to_bv (register_lookup PC sail_regs)) as [si|] eqn: Hsi.
   - move: (Hsi) => /(elem_of_dom_2 _ _ _). rewrite -Hdom. move => /elem_of_dom[ii Hii]. clear Hdom.
     have {}Hsim:= Hsim _ _ _ ltac:(done) ltac:(done) sail_regs.
     apply: raw_sim_step_i. { right. eexists _, _. by econstructor. }
@@ -649,24 +405,48 @@ Proof.
 Qed.
 
 (*** Lemmas about [sim] *)
-Lemma get_plat_config_Some_get_regval r regs x:
+Lemma get_plat_config_Some_get_regval r x:
   get_plat_config r = Some x →
-  get_regval r regs = None.
+  register_of_string r = None.
 Proof. unfold get_plat_config. repeat case_match => //. Qed.
 
-Lemma get_set_regval_config_ne r r' regs regs' v:
-  set_regval r' v regs = Some regs' →
-  r ≠ r' →
+(* TODO: Sail should generate something like this. *)
+Lemma register_of_string_roundtrip {T} (r : register T) s :
+  register_of_string s = Some (GRegister.GReg r) ->
+  string_of_register r = s.
+Proof.
+  unfold register_of_string. simpl.
+  repeat match goal with |- match (if ?eq then _ else _) with _ => _ end = _ -> _ => 
+    let H := fresh H in destruct eq eqn:H; [
+    intro H';
+    apply (inj Some) in H';
+    destruct r; try discriminate;
+    apply GRegister.greg_inj in H';
+    rewrite <- H';
+    apply String.eqb_eq in H;
+    subst;
+    reflexivity | clear H ] end.
+  discriminate.
+Qed.
+
+Lemma get_set_regval_config_ne {T} r (r' : register T) regs regs' v:
+  register_set r' v regs = regs' →
+  r ≠ string_of_register r' →
   get_regval_or_config r regs' = get_regval_or_config r regs.
 Proof.
   move => Hset Hr. rewrite /get_regval_or_config.
-  case_match as Hreg.
-  - erewrite <-get_set_regval_ne; [|done..]. by rewrite Hreg.
-  - by erewrite get_regval_None_stable.
+  destruct (register_of_string r) as [[T' r1] | ] eqn:Hreg.
+  - rewrite <- Hset. rewrite irrelevant_register_set; [reflexivity|]. 
+    rewrite register_string_eq.
+    apply Bool.not_true_is_false.
+    rewrite String.eqb_eq.
+    apply register_of_string_roundtrip in Hreg.
+    congruence.
+  - reflexivity.
 Qed.
 
 Lemma sim_done Σ:
-  sim Σ (Done tt) NilMCtx tnil.
+  sim Σ (Ret tt) NilMCtx tnil.
 Proof. move => ??????? Hdone. by apply: Hdone. Qed.
 
 Lemma sim_mctx_impl A1 A2 E1 E2 Σ e11 e12 K1 K2 e2:
@@ -695,97 +475,131 @@ Proof. move => Hsim. by apply: sim_mctx_impl. Qed.
 
 Lemma sim_pop_bind_Done A1 A2 E Σ K v f e2:
   sim (A:=A2) Σ (f v) K e2 →
-  sim (A:=A1) (E:=E) Σ (Done v) (BindMCtx f K) e2.
+  sim (A:=A1) (E:=E) Σ (Ret v) (BindMCtx f K) e2.
 Proof. move => Hsim. by apply: sim_mctx_impl. Qed.
 Lemma sim_pop_try_Done A E1 E2 Σ K v f e2:
-  sim (A:=A) (E:=E2) Σ (Done v) K e2 →
-  sim (A:=A) (E:=E1) Σ (Done v) (TryMCtx f K) e2.
+  sim (A:=A) (E:=E2) Σ (Ret v) K e2 →
+  sim (A:=A) (E:=E1) Σ (Ret v) (TryMCtx f K) e2.
 Proof. move => Hsim. by apply: sim_mctx_impl. Qed.
 
-Lemma sim_Choose {A E} Σ s ty e1 e2 K:
+(* We can't discard binds in the context until we find the try, so we'll
+   accumulate them in the term until we get a TryMCtx. *)
+Lemma sim_pop_bind_throw A1 A2 E Σ K exn f e2 :
+  sim (A:=A1) (E:=E) Σ (throw exn >>= f) K e2 →
+  sim (A:=A2) (E:=E) Σ (throw exn) (BindMCtx f K) e2.
+Proof. move => Hsim. by apply: sim_mctx_impl. Qed.
+Lemma sim_pop_binds_throw A1 A2 A3 E Σ K exn f g e2 :
+  sim (A:=A1) (E:=E) Σ (throw exn >>= (fun x : A3 => g x >>= f)) K e2 →
+  sim (A:=A2) (E:=E) Σ (throw exn >>= g) (BindMCtx f K) e2.
+Proof. move => Hsim. by apply: sim_mctx_impl. Qed.
+Lemma sim_pop_try_throw A E1 E2 Σ K exn f e2 :
+  sim (A:=A) (E:=E2) Σ (f exn) K e2 →
+  sim (A:=A) (E:=E1) Σ (throw exn) (TryMCtx f K) e2.
+Proof. move => Hsim. by apply: sim_mctx_impl. Qed.
+Lemma sim_pop_try_throw_bind A A1 E1 E2 Σ K exn f (e1 : A1 -> monad E1 A) e2 :
+  sim (A:=A) (E:=E2) Σ (f exn) K e2 →
+  sim (A:=A) (E:=E1) Σ (throw exn >>= e1) (TryMCtx f K) e2.
+Proof. move => Hsim. by apply: sim_mctx_impl. Qed.
+
+Ltac simplify_eq_dep :=
+  repeat match goal with H:@existT _ _ _ _ = @existT _ _ _ _ |- _ =>
+    let H' := fresh H in
+    specialize (eq_sigT_fst H) as H';
+    simplify_eq H';
+    apply Eqdep.EqdepTheory.inj_pair2 in H
+  end;
+  simplify_eq.
+
+Lemma sim_Choose {A E} Σ ty e1 e2 K:
   (∀ v, sim Σ (e1 v) K e2) →
-  sim (A:=A) (E:=E) Σ (Choose s ty e1) K e2.
+  sim (A:=A) (E:=E) Σ (Next (Choose ty) e1) K e2.
 Proof.
   move => Hsim ????????/=. rewrite mctx_interp_Choose.
-  apply: raw_sim_step_i. { right. eexists _, _. unshelve constructor. by apply: TypeCasts.inhabitant. }
-  move => ????/= Hstep. inversion Hstep; simplify_eq. split; [done|].
+  apply: raw_sim_step_i. { right. eexists _, _. unshelve constructor. by apply: inhabitant. }
+  move => ????/= Hstep. inversion Hstep; simplify_eq_dep. split; [done|].
   apply: raw_sim_weaken; [by apply: Hsim| lia].
 Qed.
 
-Lemma sim_Read_reg_l {A E} Σ r e1 e2 v K:
-  get_regval r Σ.(sim_regs) = Some v →
+Lemma sim_Read_reg_l {A E} Σ r ak e1 e2 v K:
+  register_lookup (T:=A) r Σ.(sim_regs) = v →
   sim Σ (e1 v) K e2 →
-  sim (A:=A) (E:=E) Σ (Read_reg r e1) K e2.
+  sim (A:=A) (E:=E) Σ (Next (RegRead r ak) e1) K e2.
 Proof.
   move => ? Hsim ????????. rewrite mctx_interp_Read_reg.
   apply: raw_sim_step_i. { right. eexists _, _. by constructor. }
-  move => ????/= Hstep. inversion Hstep; simplify_eq. split; [done|].
+  move => ????/= Hstep. inversion Hstep; simplify_eq_dep. split; [done|].
   apply: raw_sim_weaken; [by apply: Hsim| lia].
 Qed.
 
-Lemma sim_read_reg_l A E Σ (r : register_ref regstate register_value A) K e2:
-  (v' ← get_regval (name r) Σ.(sim_regs); of_regval r v') = Some (read_from r Σ.(sim_regs)) →
-  sim Σ (Done (read_from r Σ.(sim_regs))) K e2 →
-  sim (A:=A) (E:=E) Σ (read_reg r) K e2.
+Lemma sim_read_reg_ref_l A E Σ (r : register_ref register A) K e2:
+  sim Σ (Ret (register_lookup r.(reg) Σ.(sim_regs))) K e2 →
+  sim (A:=A) (E:=E) Σ (read_reg_ref r) K e2.
 Proof.
-  move => /bind_Some[rv [? Hof]] Hsim.
-  apply: sim_Read_reg_l; [done|] => ??. rewrite Hof.
+  move => Hsim.
+  apply: sim_Read_reg_l; [done|] => ??.
   by apply: Hsim.
 Qed.
 
-Lemma sim_read_reg A E Σ K e2 ann r v v':
-  get_regval (name r) Σ.(sim_regs) = Some v' →
-  of_regval r v' = Some (read_from r Σ.(sim_regs)) →
-  v = register_value_to_valu (name r) v' →
-  sim (A:=A) (E:=E) Σ (Done (read_from r Σ.(sim_regs))) K e2 →
-  sim (A:=A) (E:=E) Σ (read_reg r) K (ReadReg (name r) [] v ann :t: e2).
+Lemma sim_read_reg_l A E Σ (r : register A) K e2:
+  sim Σ (Ret (register_lookup r Σ.(sim_regs))) K e2 →
+  sim (A:=A) (E:=E) Σ (read_reg r) K e2.
 Proof.
-  move => Hget Hof -> Hsim. apply: sim_read_reg_l; [ by simplify_option_eq|].
+  move => Hsim.
+  apply: sim_Read_reg_l; [done|] => ??.
+  by apply: Hsim.
+Qed.
+
+Lemma sim_read_reg A E Σ K e2 ann r v:
+  v = register_value_to_valu r (register_lookup r Σ.(sim_regs))  →
+  sim (A:=A) (E:=E) Σ (Ret (register_lookup r Σ.(sim_regs))) K e2 →
+  sim (A:=A) (E:=E) Σ (read_reg r) K (ReadReg (string_of_register r) [] v ann :t: e2).
+Proof.
+  move => -> Hsim. apply: sim_read_reg_l.
   move => ? isla_regs ??? Hwf??.
   apply: raw_sim_safe_here => /= -[|Hsafe]. { unfold seq_to_val. by case. }
-  have [vi Hvi]: is_Some (isla_regs !! (name r)). {
+  have [vi Hvi]: is_Some (isla_regs !! (string_of_register r)). {
     move: Hsafe => [?[?[?[? Hstep]]]]. inv_seq_step. naive_solver.
   }
   apply: raw_sim_step_s. {
     econstructor. econstructor => //=. 1: by econstructor.
-    simpl. have [?[??]]:= Hwf (name r) _ ltac:(done).
-    unfold get_regval_or_config in *. simplify_option_eq.
+    simpl. have Hreg:= Hwf (string_of_register r) _ ltac:(done).
+    unfold get_regval_or_config in *. rewrite string_of_register_roundtrip in Hreg. simplify_option_eq.
     eexists _, _, _. split_and! => //. by left. }
   by apply: Hsim.
 Qed.
 
+(* The v = v' indirection allows us to use reflexivity on the get_plat_config hypothesis to
+   check that r is a config register *)
 Lemma sim_ReadReg_config A E Σ K e1 e2 ann r v v':
-  get_plat_config r = Some v' →
-  v = register_value_to_valu r v' →
+  get_plat_config r = Some v →
+  v = v' →
   sim (A:=A) (E:=E) Σ e1 K e2 →
-  sim (A:=A) (E:=E) Σ e1 K (ReadReg r [] v ann :t: e2).
+  sim (A:=A) (E:=E) Σ e1 K (ReadReg r [] v' ann :t: e2).
 Proof.
-  move => Hget -> Hsim ? isla_regs ??? Hwf??.
-  apply: raw_sim_safe_here => /= -[|Hsafe]. { unfold seq_to_val. by case. }
+  move => Hget <- Hsim ? isla_regs ??? Hwf??.
+  apply: raw_sim_safe_here => /= -[|Hsafe]. { by case. }
   have [vi Hvi]: is_Some (isla_regs !! r). {
     move: Hsafe => [?[?[?[? Hstep]]]]. inv_seq_step. naive_solver.
   }
   apply: raw_sim_step_s. {
     econstructor. econstructor => //=. 1: by econstructor.
-    simpl. have [?[Hr ?]]:= Hwf r _ ltac:(done). unfold get_regval_or_config in *.
+    simpl. have Hr:= Hwf r _ ltac:(done). unfold get_regval_or_config in *.
     erewrite get_plat_config_Some_get_regval in Hr; [|done]. simplify_option_eq.
     eexists _, _, _. split_and! => //. by left. }
   by apply: Hsim.
 Qed.
 
-Lemma sim_write_reg {A E} Σ (r : register_ref _ _ A) e2 v K v' ann:
-  name r ≠ "tlb48" ∧ name r ≠ "tlb39" →
-  set_regval (name r) (regval_of r v) Σ.(sim_regs) = Some (write_to r v Σ.(sim_regs)) →
-  v' = register_value_to_valu (name r) (regval_of r v) →
-  sim (Σ <|sim_regs := write_to r v Σ.(sim_regs)|>) (Done tt) K e2 →
-  sim (E:=E) Σ (write_reg r v) K (WriteReg (name r) [] v' ann :t: e2).
+Lemma sim_write_reg {A E} Σ (r : register A) e2 v K v' ann:
+  v' = register_value_to_valu r v →
+  sim (Σ <|sim_regs := register_set r v Σ.(sim_regs)|>) (Ret tt) K e2 →
+  sim (E:=E) Σ (write_reg r v) K (WriteReg (string_of_register r) [] v' ann :t: e2).
 Proof.
   destruct Σ => /=.
-  move => ? Hset -> Hsim ? isla_regs ? ?? Hwf ? Hdone. rewrite mctx_interp_Write_reg.
+  move => -> Hsim ? isla_regs ? ?? Hwf ? Hdone. rewrite mctx_interp_Write_reg.
   apply: raw_sim_step_i. { right. eexists _, _. by constructor. }
-  move => ????/= Hstep. inversion_clear Hstep; simplify_eq. split; [done|].
+  move => ????/= Hstep. inversion Hstep; clear Hstep; simplify_eq_dep. split; [done|].
   apply: raw_sim_safe_here => /= -[|Hsafe]. { unfold seq_to_val. by case. }
-  have [vi Hvi]: is_Some (isla_regs !! (name r)). {
+  have [vi Hvi]: is_Some (isla_regs !! (string_of_register r)). {
     move: Hsafe => [?[?[?[? Hstep]]]]. inv_seq_step. naive_solver.
   }
   apply: raw_sim_step_s. {
@@ -793,9 +607,9 @@ Proof.
     eexists _, _, _. done.
   }
   apply: raw_sim_weaken; [apply Hsim => /=| ].
-  - move => r' vi'. destruct (decide (r' = name r)); simplify_eq.
-    + rewrite lookup_insert. move: Hset => /get_set_regval.
-      unfold get_regval_or_config => ->; naive_solver.
+  - move => r' vi'. destruct (decide (r' = string_of_register r)); simplify_eq.
+    + rewrite lookup_insert. move => [?].
+      unfold get_regval_or_config. rewrite string_of_register_roundtrip register_lookup_set. naive_solver.
     + rewrite lookup_insert_ne //.
       erewrite get_set_regval_config_ne; [|done..]. by apply: Hwf.
   - apply/lookup_insert_None. unfold private_regs_wf in *.
@@ -804,23 +618,21 @@ Proof.
   - lia.
 Qed.
 
-Lemma sim_write_reg_private {A E} Σ (r : register_ref _ _ A) e2 v K:
-  set_regval (name r) (regval_of r v) Σ.(sim_regs) = Some (write_to r v Σ.(sim_regs)) →
-  name r = "nextPC" →
-  sim (Σ <|sim_regs := write_to r v Σ.(sim_regs)|>) (Done tt) K e2 →
+Lemma sim_write_reg_private {E} Σ (r : register _) e2 v K:
+  r = nextPC →
+  sim (Σ <|sim_regs := register_set r v Σ.(sim_regs)|>) (Ret tt) K e2 →
   sim (E:=E) Σ (write_reg r v) K e2.
 Proof.
   destruct Σ => /=.
-  move => Hset Heq Hsim ? isla_regs ? ?? Hwf ? Hdone. rewrite mctx_interp_Write_reg.
+  move => Heq Hsim ? isla_regs ? ?? Hwf ? Hdone. rewrite mctx_interp_Write_reg.
   apply: raw_sim_step_i. { right. eexists _, _. by constructor. }
-  move => ????/= Hstep. inversion_clear Hstep; simplify_eq. split; [done|].
+  move => ????/= Hstep. inversion Hstep; clear Hstep; simplify_eq_dep. split; [done|].
   apply: raw_sim_weaken; [apply Hsim => /=; [|done..]| lia].
-  move => ?? Hisla. have [?[??]]:= Hwf _ _ ltac:(done).
-  eexists _. split; [|done].
-  erewrite get_set_regval_config_ne; [done..|].
-  move => ?. subst. unfold private_regs_wf in *. rewrite Heq in Hisla. naive_solver.
+  move => ?? Hisla. have ?:= Hwf _ _ ltac:(done).
+  erewrite get_set_regval_config_ne with (r' := nextPC) (v := v) (regs := sim_regs0); [done..|].
+  move => Hnotpc. compute in Hnotpc. subst. unfold private_regs_wf in *. congruence.
 Qed.
-
+(*
 Lemma sim_Write_ea {A E} Σ e1 e2 K n2 n1 wk:
   sim Σ e1 K e2 →
   sim (A:=A) (E:=E) Σ (Write_ea wk n1 n2 e1) K e2.
@@ -830,20 +642,22 @@ Proof.
   move => ????/= Hstep. inversion Hstep; simplify_eq. split; [done|].
   apply: raw_sim_weaken; [by apply: Hsim| lia].
 Qed.
+*)
 
-Lemma sim_write_mem {E} Σ e2 n' (sz : Z) (v : mword (8 * sz)) K (v' : bv n') ann res wk' (a : mword 64) (a' : addr) len' d:
+Lemma sim_write_mem {E} Σ e2 n' (sz : Z) K (v' : bv n') ann res wk' (a' : addr) len' v req:
   (8 * len' = n')%N →
   sz = Z.of_N len' →
   res = RVal_Bool true →
-  mword_to_bv a = a' →
+  req.(ConcurrencyInterfaceTypes.Mem_write_request_pa) = a' →
+  req.(ConcurrencyInterfaceTypes.Mem_write_request_value) = Some v →
   mword_to_bv v = v' →
-  sim Σ (Done true) K e2 →
-  sim (E:=E) Σ (Prompt_monad.write_mem Write_plain d a sz v) K (WriteMem res wk' (RVal_Bits a') (RVal_Bits v') len' None ann :t: e2).
+  sim Σ (Ret (Ok None)) K e2 →
+  sim (E:=E) Σ (sail_mem_write (n := sz) req) K (WriteMem res wk' (RVal_Bits a') (RVal_Bits v') len' None ann :t: e2).
 Proof.
-  move => ? ? ? ? ? Hsim ? isla_regs mem ?? Hwf ? Hdone. subst.
-  set a' := mword_to_bv a. set v' := mword_to_bv (n2:=8 * len') v.
-  unfold Prompt_monad.write_mem. simplify_option_eq.
-  erewrite mem_bytes_of_bits_to_bv; [|done|lia].
+  move => ? ? ? ? ? ? Hsim ? isla_regs mem ?? Hwf ? Hdone. subst.
+  set a' := ConcurrencyInterfaceTypes.Mem_write_request_pa req.
+  set v' := mword_to_bv (n2:=8 * len') v.
+  unfold sail_mem_write. simplify_option_eq.
   rewrite mctx_interp_Write_mem.
   apply: raw_sim_safe_here => /= -[|Hsafe]. { unfold seq_to_val. by case. }
   have {Hsafe}[? Hor] : 0 < Z.of_N len' ∧ (is_Some (read_mem_list mem (bv_unsigned a') len') ∨
@@ -857,17 +671,19 @@ Proof.
     + move: Hmem => /fmap_Some. naive_solver.
     + move: Hmem => /fmap_None. naive_solver.
   }
-  have Heq : Z.of_N (Word.wordToN a) = bv_unsigned a'.
-  { rewrite mword_to_bv_unsigned //. }
-  have Heq2 : (bv_unsigned (mword_to_bv (n2:=(Z.to_N (8 * Z.of_N len'))) v) = (bv_unsigned v')).
-  { rewrite /v' !mword_to_bv_unsigned //; lia. }
   constructor => _. split. {
     right. move: Hor => [[? Hm]//|[Hm [??]]].
     all: eexists _, _; eapply SailWriteMem; [done..|].
-    all: by rewrite !Z_nat_N !N2Z.id !Heq Z_to_bv_bv_unsigned Hm.
+    all: rewrite /= {1}N2Z.id Hm ?Z2N.id; [> done | done | by apply N2Z.is_nonneg].
   }
-  move => ? ? ? ? Hstep. inversion_clear Hstep; simplify_eq.
-  move: H2. rewrite !Z_nat_N !N2Z.id !Heq Z_to_bv_bv_unsigned.
+  move => ? ? ? ? Hstep. inversion Hstep; simplify_eq_dep; clear Hstep.
+  move: H7. rewrite /= {1}N2Z.id. (*rewrite !Z_nat_N !N2Z.id !Heq Z_to_bv_bv_unsigned.*)
+
+  unfold mword_to_bv in v'.
+  generalize (sail_mem_write_subproof (Z.of_N len')).
+  rewrite N2Z.id /= => EQ_len.
+  rewrite (N_eq_dec_eq _ _ EQ_len) in v' |- *.
+
   move: Hor => [[? Hm]//|[Hm ?]]; rewrite Hm.
   - move => [??]. simplify_eq. eexists _. split. {
       apply: (steps_l' _ _ _ _ _ []); [ |by apply: steps_refl| by rewrite right_id_L].
@@ -875,33 +691,29 @@ Proof.
       eexists _, _, v'. split_and! => //.
       by rewrite /read_mem Hm.
     }
-    rewrite /write_mem N_nat_Z Heq2.
-    apply: raw_sim_weaken; [by apply Hsim| lia].
+    apply: raw_sim_weaken; [by apply Hsim | lia].
   - move => [?[?[??]]]. simplify_eq. eexists _. split. {
       apply: (steps_l' _ _ _ _ _ []); [ |by apply: steps_refl| by rewrite right_id_L].
       econstructor. econstructor; [done| by econstructor|] => /=.
       eexists _, _, v'. split_and! => //.
       rewrite /read_mem Hm /=. split_and! => //.
-      rewrite Heq2 Z_to_bv_little_endian_to_bv_to_little_endian //; lia.
     }
     apply: raw_sim_weaken; [by apply Hsim| lia].
     Unshelve. apply: inhabitant.
 Qed.
 
-Lemma sim_read_mem {E} Σ (sz : Z) e2 K ann ann' rk' (a : mword 64) (a' : addr) len' len'' d sm:
+Lemma sim_read_mem {E} Σ (sz : Z) e2 K ann ann' rk' (a' : addr) len' len'' sm req:
   len'' = (8 * len')%N →
   sz = Z.of_N len' →
-  mword_to_bv a = a' →
-  (∀ r1 (r2 : bv len''), r1 = bv_to_mword r2 → sim Σ (Done r1) K (subst_trace (Val_Bits r2) sm e2)) →
-  sim (E:=E) Σ (Prompt_monad.read_mem Read_plain d a sz) K
+  req.(ConcurrencyInterfaceTypes.Mem_read_request_pa) = a' →
+  (∀ r1 (r2 : bv len''), r1 = bv_to_mword r2 → sim Σ ((Ret (Ok (r1, None)))) K (subst_trace (Val_Bits r2) sm e2)) →
+  sim (E:=E) Σ (sail_mem_read (n := sz) req) K
       (Smt (DeclareConst sm (Ty_BitVec len'')) ann' :t:
        ReadMem (RVal_Symbolic sm) rk' (RVal_Bits a') len' None ann :t: e2).
 Proof.
-  move => ? ? ? Hsim. subst. set a' := mword_to_bv a.
-  unfold Prompt_monad.read_mem, read_mem_bytes. apply sim_bind.
+  move => ? ? ? Hsim. subst. set a' := ConcurrencyInterfaceTypes.Mem_read_request_pa req.
+  unfold sail_mem_read, read_mem_bytes.
   move => ? isla_regs mem ?? Hwf ? Hdone. rewrite mctx_interp_Read_mem.
-  have Heq : Z.of_N (Word.wordToN a) = bv_unsigned a'.
-  { rewrite mword_to_bv_unsigned //. }
   constructor => Hsafe.
   have {Hsafe}[? Hor] : 0 < Z.of_N len' ∧ (is_Some (read_mem_list mem (bv_unsigned a') len') ∨
     (read_mem_list mem (bv_unsigned a') len' = None ∧
@@ -920,15 +732,14 @@ Proof.
   }
   split. {
     right. move: Hor => [[? Hm]//|[Hm [??]]].
-    all: eexists _, _; eapply SailReadMem; [done..| | by rewrite !Z_nat_N !N2Z.id !Heq Z_to_bv_bv_unsigned Hm].
-    - move: Hm => /mapM_Some /Forall2_length <-. rewrite seqZ_length. lia.
-    - apply replicate_length.
+    all: eexists _, _; eapply SailReadMem; rewrite /= {1}N2Z.id Hm ?Z2N.id; [> done.. | by apply N2Z.is_nonneg ].
   }
-  move => ? ? ? ? Hstep. inversion_clear Hstep; simplify_eq.
-  move: H2. rewrite !Z_nat_N !N2Z.id !Heq Z_to_bv_bv_unsigned.
-  rewrite (read_mem_bytes_eq len') /=.
-  2: { rewrite H1. lia. } 2: { rewrite H1. lia. }
-  move: Hor => [[? Hm]//|[Hm ?]]; rewrite Hm.
+  (* Get this rewrite out of the way before we introduce any evars *)
+  generalize (sail_mem_read_subproof (Z.of_N len')) => PF.
+  rewrite N2Z.id in PF |- *.
+  move => ? ? ? ? Hstep. inversion Hstep; simplify_eq_dep; clear Hstep.
+  move: H8.
+  move: Hor => [[? Hm]//|[Hm [??]]]; rewrite Hm.
   - move => [??]. simplify_eq. eexists _. split. {
       apply: steps_l'.
       { econstructor. econstructor; [done| eapply DeclareConstBitVecS' |] => /=. done. } 2: done.
@@ -937,7 +748,9 @@ Proof.
       eexists _, _, _. split_and! => //. { by rewrite /eq_var_name Z.eqb_refl. }
       rewrite /read_mem Hm/=. split_and! => //. by left.
     }
-    apply: raw_sim_weaken; [by apply Hsim|lia].
+    apply: raw_sim_weaken; [apply Hsim; [ | done..] | lia].
+    unfold bv_to_mword.
+    by rewrite N_eq_dec_eq.
   - move => [?[??]]. simplify_eq. eexists _. split. {
       apply: steps_l'.
       { econstructor. econstructor; [done| apply: DeclareConstBitVecS'; shelve|] => /=. done. } 2: done.
@@ -946,19 +759,21 @@ Proof.
       eexists _, _, _. split_and! => //. { by rewrite /eq_var_name Z.eqb_refl. }
       by rewrite /read_mem Hm/=.
     }
-    apply: raw_sim_weaken; [by apply Hsim| lia].
+    apply: raw_sim_weaken; [apply Hsim; [ | done..]| lia].
+    unfold bv_to_mword.
+    by rewrite N_eq_dec_eq.
     Unshelve. all: apply inhabitant.
 Qed.
 
 Lemma sim_assert_exp' E Σ b K e2 s:
   b = true →
-  (∀ H, sim Σ (Done H) K e2) →
+  (∀ H, sim Σ (Ret H) K e2) →
   sim (E:=E) Σ (assert_exp' b s) K e2.
-Proof. move => Hb Hsim. unfold assert_exp'. destruct b => //. Qed.
+Proof. move => Hb Hsim. unfold assert_exp'. destruct b => //. by unfold returnm. Qed.
 
 Lemma sim_assert_exp E Σ b K e2 s:
   b = true →
-  sim Σ (Done tt) K e2 →
+  sim Σ (Ret tt) K e2 →
   sim (E:=E) Σ (assert_exp b s) K e2.
 Proof. move => Hb Hsim. unfold assert_exp. destruct b => //. Qed.
 
@@ -1040,7 +855,7 @@ Qed.
 Definition eval_assume_val' (regs : regstate) (v : assume_val) : option base_val :=
   match v with
   | AVal_Var r l => v' ← get_regval_or_config r regs;
-                   v'' ← read_accessor l (register_value_to_valu r v');
+                   v'' ← read_accessor l v';
                    if v'' is RegVal_Base b then Some b else None
   | AVal_Bool b => Some (Val_Bool b)
   | AVal_Bits b => Some (Val_Bits b)
@@ -1070,7 +885,7 @@ Lemma eval_assume_val'_sound isla_regs sail_regs e v:
 Proof.
   destruct e => //=.
   move => /bind_Some[?[? ?]] Hwf.
-  have [?[-> ?]]:= Hwf _ _ ltac:(done). by subst.
+  have ->:= Hwf _ _ ltac:(done). by subst.
 Qed.
 
 Lemma eval_a_exp'_sound isla_regs sail_regs e v:
@@ -1106,7 +921,7 @@ Proof.
 Qed.
 
 Lemma sim_AssumeReg A E Σ K e1 e2 ann r v al:
-  ((v' ← get_regval_or_config r Σ.(sim_regs); read_accessor al (register_value_to_valu r v')) = Some v
+  ((v' ← get_regval_or_config r Σ.(sim_regs); read_accessor al v') = Some v
     → sim (A:=A) (E:=E) Σ e1 K e2) →
   sim (A:=A) (E:=E) Σ e1 K (AssumeReg r al v ann :t: e2).
 Proof.
@@ -1115,6 +930,6 @@ Proof.
   revert select (∃ v, _) => -[?[?[?[?[??]]]]]. simplify_eq.
   apply: raw_sim_step_s. { econstructor. econstructor => //=. 1: by econstructor. naive_solver. }
   apply: Hsim; [|done..].
-  have [?[??]]:= Hwf r _ ltac:(done). simplify_eq.
+  have ?:= Hwf r _ ltac:(done). simplify_eq.
   apply/bind_Some. naive_solver.
 Qed.
