sail-riscv/memcpy.v
@@ -53,35 +53,35 @@
 (* Exceptions to this license are detailed in THIRD_PARTY_FILES.md          *)
 (****************************************************************************)
 
-Require Import Sail.Base.
-Require Import Sail.State_monad.
-Require Import Sail.State_lifting.
+Require Import SailStdpp.Base.
 Require Import isla.sail_riscv.sail_opsem.
 Require Import isla.sail_riscv.tactics.
 Require Import isla.automation.
 Require Import isla.riscv64.riscv64.
 From isla.instructions.memcpy_riscv64 Require Import instrs.
 
+(* Workaround for unification problem, will upstream to stdpp *)
+Global Hint Extern 10 (BvUnfold _ _ _ (@BV _ _ _) _) => apply bv_unfold_BV : bv_unfold_db.
+
 Lemma sim_instr_a0:
   sim_instr (Uncompressed (BV 32 0x00060e63)) a0.
 Proof.
   move => regs. unfold step_cpu, a0.
   red_sim. unfold execute. red_sim. unfold execute_BTYPE.
-  red_sim.
-  apply: sim_read_reg_l; [done|]. red_sim. rewrite x12_nextPC.
-  destruct (eq_vec (x12 regs) zero_reg) eqn: Hx12; sim_simpl_hyp Hx12; red_sim.
+  red_sim. apply: sim_read_reg_l. red_sim. sim_simpl_regs.
+  destruct (eq_vec (register_lookup (T:=regtype) x12 regs) zero_reg) eqn: Hx12; sim_simpl_hyp Hx12; red_sim.
   - apply: (sim_tcases 0); [done|]. red_sim.
     rewrite bit_to_bool_false; [|shelve]. red_sim.
   - apply: (sim_tcases 1); [done|]. red_sim.
   Unshelve. all: sim_simpl_goal.
-  + rewrite (eq_vec_to_bv 64) // bool_decide_eq_true in Hx12. by rewrite Hx12.
+  + rewrite /get_word in Hx12. reduce_closed zero_reg. rewrite Hx12. by bv_solve.
   + rewrite access_vec_dec_to_bv // bitU_of_bool_B0 //.
     rewrite mword_to_bv_add_vec //=. reduce_closed_mword_to_bv.
     bv_simplify. rename select (bv_extract 1 _ _ = _) into He. bv_simplify He.
     bitblast. by bitblast He with 0.
-  + rewrite mword_to_bv_add_vec //.
-  + rewrite (eq_vec_to_bv 64) // bool_decide_eq_false in Hx12. done.
-  + rewrite mword_to_bv_add_vec //.
+  + rewrite /mword_to_bv/=.
+    contradict Hx12. rewrite /get_word. reduce_closed zero_reg.
+    rewrite Hx12. apply bv_eq. reflexivity.
 Qed.
 
 Lemma sim_instr_a4:
@@ -90,34 +90,29 @@ Proof.
   move => regs. unfold step_cpu, a4.
   red_sim. unfold execute. red_sim. unfold execute_LOAD. red_sim.
   rewrite if_false; [|shelve]. red_sim.
-  unfold translateAddr. red_sim. rewrite mstatus_nextPC cur_privilege_nextPC.
+  unfold translateAddr. red_sim. sim_simpl_regs.
   apply sim_effectivePrivilege; [done|]. red_sim.
-  unfold translateAddr_priv. red_sim.
-  apply: sim_read_reg_l; [solve_of_regval_regval_of|]. red_sim.
-  apply: sim_read_reg_l; [solve_of_regval_regval_of|]. red_sim.
   unfold translationMode.
-  have -> : (cur_privilege regs) = Machine by destruct (cur_privilege regs). red_sim.
-  apply: sim_read_reg_l; [solve_of_regval_regval_of|]. red_sim. rewrite x11_nextPC.
+  have -> : (register_lookup cur_privilege regs) = Machine by destruct (register_lookup cur_privilege regs). red_sim.
   unfold mem_read. red_sim.
-  apply: sim_read_reg_l; [solve_of_regval_regval_of|]. red_sim.
-  apply: sim_read_reg_l; [solve_of_regval_regval_of|]. red_sim. rewrite mstatus_nextPC.
+  apply: sim_read_reg_l. red_sim.
+  apply: sim_read_reg_l. red_sim. sim_simpl_regs.
   apply sim_effectivePrivilege; [done|]. red_sim.
+  unfold phys_access_check.
   rewrite Hassume. red_sim.
   rewrite if_false; [|shelve]. rewrite if_true; [|shelve]. red_sim.
   Unshelve. all: sim_simpl_goal.
   - apply check_misaligned_false. rewrite mword_to_bv_add_vec; [|done]. reduce_closed_mword_to_bv.
     by rewrite bv_unsigned_N_0.
+  - congruence.
   - eapply within_mmio_writable_false.
     + rewrite mword_to_bv_add_vec; [|done]. reduce_closed_mword_to_bv. done.
     + rewrite ->Hassume1, Hassume2, Hassume5, Hassume6, Hassume7, !bv_add_unsigned, !bv_unsigned_BV in *.
-      unfold bv_wrap, bv_modulus in *. lia.
+      unfold bv_wrap, bv_modulus in *. generalize_regs. lia.
   - eapply within_phys_mem_true.
     + rewrite mword_to_bv_add_vec; [|done]. reduce_closed_mword_to_bv. done.
     + rewrite ->Hassume1, Hassume2, !bv_add_unsigned, !bv_unsigned_BV in *.
-      unfold bv_wrap, bv_modulus in *. lia.
-  - by rewrite mword_to_bv_add_vec.
-  - rewrite mword_to_bv_sign_extend' // mword_to_bv_to_mword //.
-  - rewrite mword_to_bv_add_vec //.
+      unfold bv_wrap, bv_modulus in *. generalize_regs. lia.
     Unshelve. all: exact: inhabitant.
 Qed.
 
@@ -127,34 +122,31 @@ Proof.
   move => regs. unfold step_cpu, a8.
   red_sim. unfold execute. red_sim. unfold execute_STORE.  red_sim.
   rewrite if_false; [|shelve]. red_sim.
-  unfold translateAddr. red_sim. rewrite mstatus_nextPC cur_privilege_nextPC.
+  unfold translateAddr. red_sim. sim_simpl_regs.
   apply sim_effectivePrivilege; [done|]. red_sim.
-  unfold translateAddr_priv. red_sim.
-  apply: sim_read_reg_l; [solve_of_regval_regval_of|]. red_sim.
-  apply: sim_read_reg_l; [solve_of_regval_regval_of|]. red_sim.
   unfold translationMode.
-  have -> : (cur_privilege regs) = Machine by destruct (cur_privilege regs). red_sim.
-  apply: sim_read_reg_l; [solve_of_regval_regval_of|]. red_sim. rewrite x10_nextPC.
+  have -> : (register_lookup cur_privilege regs) = Machine by destruct (register_lookup cur_privilege regs).  red_sim.
+  unfold write_kind_of_flags. red_sim.
   unfold mem_write_value, mem_write_value_meta. red_sim.
-  apply: sim_read_reg_l; [solve_of_regval_regval_of|]. red_sim.
-  apply: sim_read_reg_l; [solve_of_regval_regval_of|]. red_sim. rewrite mstatus_nextPC cur_privilege_nextPC.
+  apply: sim_read_reg_l. red_sim.
+  apply: sim_read_reg_l. red_sim. sim_simpl_regs.
   apply sim_effectivePrivilege; [done|]. red_sim.
-  rewrite Hassume. red_sim.
+  unfold phys_access_check. rewrite Hassume. red_sim.
   rewrite if_false; [|shelve]. rewrite if_true; [|shelve]. red_sim.
+  unfold write_kind_of_flags. red_sim.
+  unfold ext_check_phys_mem_write. red_sim.
   Unshelve. all: sim_simpl_goal.
   - apply check_misaligned_false. rewrite mword_to_bv_add_vec; [|done]. reduce_closed_mword_to_bv.
     by rewrite bv_unsigned_N_0.
+  - congruence.
   - eapply within_mmio_writable_false.
     + rewrite mword_to_bv_add_vec; [|done]. reduce_closed_mword_to_bv. done.
     + rewrite ->Hassume1, Hassume2, Hassume5, Hassume6, Hassume7, !bv_add_unsigned, !bv_unsigned_BV in *.
-      unfold bv_wrap, bv_modulus in *. lia.
+      unfold bv_wrap, bv_modulus in *. generalize_regs. lia.
   - eapply within_phys_mem_true.
     + rewrite mword_to_bv_add_vec; [|done]. reduce_closed_mword_to_bv. done.
     + rewrite ->Hassume1, Hassume2, !bv_add_unsigned, !bv_unsigned_BV in *.
-      unfold bv_wrap, bv_modulus in *. lia.
-  - by rewrite mword_to_bv_add_vec.
-  - by rewrite (mword_to_bv_subrange_vec_dec 7 0 64).
-  - by rewrite mword_to_bv_add_vec.
+      unfold bv_wrap, bv_modulus in *. generalize_regs. lia.
     Unshelve. all: exact: inhabitant.
 Qed.
 
@@ -165,8 +157,6 @@ Proof.
   red_sim. unfold execute. red_sim. unfold execute_ITYPE.
   red_sim.
   Unshelve. all: sim_simpl_goal.
-  - by rewrite mword_to_bv_add_vec.
-  - by rewrite mword_to_bv_add_vec.
 Qed.
 
 Lemma sim_instr_a10:
@@ -195,20 +185,21 @@ Proof.
   move => regs. unfold step_cpu, a18.
   red_sim. unfold execute. red_sim. unfold execute_BTYPE.
   red_sim.
-  apply: sim_read_reg_l; [solve_of_regval_regval_of|]. red_sim. rewrite x12_nextPC.
-  destruct (neq_vec (x12 regs) zero_reg) eqn: Hx12; unfold neq_vec in Hx12; sim_simpl_hyp Hx12; red_sim.
+  apply: sim_read_reg_l. red_sim. sim_simpl_regs.
+  destruct (neq_vec (@register_lookup regtype x12 regs) zero_reg) eqn: Hx12; unfold neq_vec in Hx12; sim_simpl_hyp Hx12; red_sim.
   - apply: (sim_tcases 0); [done|]. red_sim.
     rewrite bit_to_bool_false; [|shelve]. red_sim.
   - apply: (sim_tcases 1); [done|]. red_sim.
   Unshelve. all: sim_simpl_goal.
-  + rewrite (eq_vec_to_bv 64) // bool_decide_eq_false in Hx12. contradict Hx12. by rewrite Hx12.
+  + rewrite /mword_to_bv/=. contradict Hx12.
+    rewrite /get_word Hx12. apply bv_eq. done.
   + rewrite access_vec_dec_to_bv // bitU_of_bool_B0 //.
     rewrite mword_to_bv_add_vec //=. reduce_closed_mword_to_bv.
     bv_simplify. rename select (bv_extract 1 _ _ = _) into He. bv_simplify He.
     bitblast. by bitblast He with 0.
-  + rewrite mword_to_bv_add_vec //.
-  + rewrite (eq_vec_to_bv 64) // bool_decide_eq_true in Hx12. done.
-  + rewrite mword_to_bv_add_vec //.
+  + rewrite /get_word in Hx12.
+    rewrite Hx12. reduce_closed_mword_to_bv.
+    by apply bv_eq.
 Qed.
 
 Lemma sim_instr_a1c:
